pmatch versions of various functions
For issue #136

compiler/backend/bvl_constScript.sml
@@ -2,6 +2,7 @@ open preamble bvlTheory
 
 val _ = new_theory "bvl_const";
 
+val _ = patternMatchesLib.ENABLE_PMATCH_CASES();
 (*
 
    This is a BVL transformation that propagates simple and
@@ -23,15 +24,27 @@ val dest_simple_def = Define `
   (dest_simple _ = NONE)`;
 val _ = export_rewrites["dest_simple_def"];
 
-val SmartOp_def = Define `
+val dest_simple_pmatch = Q.store_thm("dest_simple_pmatch",`
+  ∀op. dest_simple op =
+    case op of
+      bvl$Op (Const i) [] => SOME i
+    | _ => NONE`
+  ho_match_mp_tac (theorem "dest_simple_ind")
+  >> rpt strip_tac
+  >> PURE_ONCE_REWRITE_TAC [dest_simple_def]
+  >- (Cases_on `xs` >> fs[])
+  >> CONV_TAC(RAND_CONV patternMatchesLib.PMATCH_SIMP_CONV)
+  >> REFL_TAC)
+
+val SmartOp_quotation = `
   SmartOp op (xs:bvl$exp list) =
     let default = Op op xs in
-      case xs of
+      dtcase xs of
       | [x1;x2] =>
         if MEM op [Add; Sub; Mult; Div; Mod; Less; LessEq; Greater; GreaterEq] then
-          case (dest_simple x1, dest_simple x2) of
+          dtcase (dest_simple x1, dest_simple x2) of
           | (SOME x2, SOME (x1:int)) =>
-              (case op of
+              (dtcase op of
                | Add => Op (Const (x1 + x2)) []
                | Sub => Op (Const (x1 - x2)) []
                | Mult => Op (Const (x1 * x2)) []
@@ -44,7 +57,7 @@ val SmartOp_def = Define `
                | _ => default)
           | _ => default
         else if op = Equal then
-          case (dest_simple x2, dest_simple x1) of
+          dtcase (dest_simple x2, dest_simple x1) of
           | (SOME i, SOME j) => Bool (i = j)
           | (SOME i, _) => Op (EqualInt i) [x1]
           | (_, SOME i) => Op (EqualInt i) [x2]
@@ -52,12 +65,49 @@ val SmartOp_def = Define `
         else default
       | _ => default`
 
+val SmartOp_def = Define SmartOp_quotation
+
+val SmartOp_pmatch = Q.store_thm("SmartOp_pmatch",
+  SmartOp_quotation |>
+   map (fn QUOTE s => Portable.replace_string {from="dtcase",to="case"} s |> QUOTE
+       | aq => aq),
+      rpt strip_tac
+      >> PURE_ONCE_REWRITE_TAC [SmartOp_def]
+      >> PURE_REWRITE_TAC [LET_DEF]
+      >> BETA_TAC
+      >> CONV_TAC patternMatchesLib.PMATCH_LIFT_BOOL_CONV
+      >> PURE_TOP_CASE_TAC
+      >> CONV_TAC(RATOR_CONV(RAND_CONV(CASE_SIMP_CONV)))
+      >> RW_TAC std_ss[MEM]
+      >> TRY (CONV_TAC patternMatchesLib.PMATCH_LIFT_BOOL_CONV)
+      >> PURE_TOP_CASE_TAC
+      >> CONV_TAC(RATOR_CONV(RAND_CONV(CASE_SIMP_CONV)))
+      >> SIMP_TAC std_ss[]
+      >> every_case_tac
+      >> FULL_SIMP_TAC std_ss[fetch "patternMatches" "PMATCH_INCOMPLETE_def"])
+
 val extract_def = Define `
   (extract ((Var n):bvl$exp) ys = SOME ((Var (n + LENGTH ys + 1)):bvl$exp)) /\
   (extract (Op (Const i) xs) ys = SOME (Op (Const i) [])) /\
   (extract (Op (Cons t) xs) ys =
     if NULL xs then SOME (Op (Cons t) []) else NONE) /\
   (extract _ _ = NONE)`
+
+val extract_pmatch = Q.store_thm("extract_pmatch",`
+  ∀op ys. extract op ys =
+    case op of
+      (Var n):bvl$exp => SOME ((Var (n + LENGTH ys + 1)):bvl$exp)
+    | Op (Const i) xs => SOME (Op (Const i) [])
+    | Op (Cons t) [] => SOME (Op (Cons t) [])
+    | _ => NONE`,
+  ho_match_mp_tac (theorem "extract_ind")
+  >> rpt strip_tac
+  >> PURE_ONCE_REWRITE_TAC [extract_def]
+  >> CONV_TAC(RAND_CONV patternMatchesLib.PMATCH_SIMP_CONV)
+  >> TRY REFL_TAC
+  >> PURE_ONCE_REWRITE_TAC [NULL_EQ]
+  >> Cases_on `xs`
+  >> fs[])
 
 val extract_list_def = Define `
   (extract_list [] = []) /\
@@ -67,11 +117,22 @@ val delete_var_def = Define `
   (delete_var ((Var n):bvl$exp) = Op (Const 0) []) /\
   (delete_var x = x)`;
 
+val delete_var_pmatch = Q.store_thm("delete_var_pmatch",`!op.
+  delete_var op =
+    case op of
+      Var n => Op (Const 0) []
+    | x => x`,
+  ho_match_mp_tac (theorem "delete_var_ind")
+  >> rpt strip_tac
+  >> PURE_ONCE_REWRITE_TAC [delete_var_def]
+  >> CONV_TAC(RAND_CONV patternMatchesLib.PMATCH_SIMP_CONV)
+  >> REFL_TAC)
+
 val compile_def = tDefine "compile" `
   (compile env [] = []) /\
   (compile env (x::y::xs) = compile env [x] ++ compile env (y::xs)) /\
   (compile env [Var v] =
-     case LLOOKUP env v of
+     dtcase LLOOKUP env v of
      | NONE => [Var v]
      | SOME NONE => [Var v]
      | SOME (SOME (Var i)) => [Var (v + i)]
@@ -94,7 +155,7 @@ val compile_def = tDefine "compile" `
   (compile env [Op op xs] = [SmartOp op (compile env xs)]) /\
   (compile env [Tick x] = [Tick (HD (compile env [x]))]) /\
   (compile env [Call t dest xs] = [Call t dest (compile env xs)])`
- (WF_REL_TAC `measure (exp1_size o SND)`);
+  (WF_REL_TAC `measure (exp1_size o SND)`);
 
 val compile_ind = theorem"compile_ind";
 
@@ -110,6 +171,6 @@ val compile_HD_SING = Q.store_thm("compile_HD_SING",
   \\ Cases_on `compile n [x]` \\ fs [LENGTH_NIL]);
 
 val compile_exp_def = Define `
-  compile_exp x = case compile [] [x] of (y::_) => y | _ => Var 0 (* impossible *)`;
+  compile_exp x = dtcase compile [] [x] of (y::_) => y | _ => Var 0 (* impossible *)`;
 
 val _ = export_theory();
