compiler/inference/inferScript.sml
@@ -12,6 +12,28 @@ val _ = save_thm("inf_type_to_string_def",inf_type_to_string_def);
 val _ = save_thm("inf_type_to_string_ind",inf_type_to_string_ind);
 val _ = computeLib.add_persistent_funs ["inf_type_to_string_def"];
 
+val inf_type_to_string_pmatch = Q.store_thm("inf_type_to_string_pmatch",`
+ (∀t. inf_type_to_string t =
+    case t of
+      Infer_Tuvar _ => "<unification variable>"
+    | Infer_Tvar_db n => num_to_dec_string n
+    | Infer_Tapp [t1;t2] TC_fn =>
+       STRCAT"("  (STRCAT(inf_type_to_string t1)  (STRCAT"->"  (STRCAT(inf_type_to_string t2) ")")))
+    | Infer_Tapp _ TC_fn => "<bad function type>"
+    | Infer_Tapp ts TC_tup => (STRCAT"("  (STRCAT(inf_types_to_string ts) ")"))
+    | Infer_Tapp [] tc1 => tc_to_string tc1
+    | Infer_Tapp ts tc1 => STRCAT"("  (STRCAT(inf_types_to_string ts)  (STRCAT") " (tc_to_string tc1)))) /\
+ (∀ts. inf_types_to_string ts =
+    case ts of
+      [] => ""
+    | [t] => inf_type_to_string t
+    | t::ts => STRCAT(inf_type_to_string t)  (STRCAT", " (inf_types_to_string ts)))`,
+  ho_match_mp_tac inf_type_to_string_ind
+  >> rpt strip_tac
+  >> PURE_ONCE_REWRITE_TAC [inf_type_to_string_def]
+  >> CONV_TAC(RAND_CONV patternMatchesLib.PMATCH_SIMP_CONV)
+  >> REFL_TAC);
+
 val list_subset_def = Define `
 list_subset l1 l2 = EVERY (\x. MEM x l2) l1`;
 
@@ -403,7 +425,7 @@ constrain_op op ts =
 
 val constrain_op_def = Define constrain_op_quotation
 
-val constrain_op_pmatch = Q.prove(`∀op ts.` @
+val constrain_op_pmatch = Q.store_thm("constrain_op_pmatch",`∀op ts.` @
   (constrain_op_quotation |>
    map (fn QUOTE s => Portable.replace_string {from="dtcase",to="case"} s |> QUOTE
        | aq => aq)),
